

Factoring Monic Quadratics

Today we focus only on the factors.

1. Both Factors Positive

Positive constant \rightarrow same-sign factors. Linear term positive \rightarrow both factors positive.

a)

$$x^2 + 3x + 2 = 0$$

$$(x + 1)(x + 2)$$

b)

$$x^2 + 5x + 6 = 0$$

$$(x + 2)(x + 3)$$

c)

$$x^2 + 6x + 5 = 0$$

$$(x + 1)(x + 5)$$

d)

$$x^2 + 7x + 12 = 0$$

$$(x + 3)(x + 4)$$

e)

$$x^2 + 11x + 28 = 0$$

$$(x + 4)(x + 7)$$

f)

$$x^2 + 14x + 45 = 0$$

$$(x + 5)(x + 9)$$

2. Both Factors Negative

Positive constant \rightarrow same-sign factors. Linear term negative \rightarrow both factors negative.

a)

$$x^2 - 3x + 2 = 0$$

$$(x - 1)(x - 2)$$

b)

$$x^2 - 6x + 5 = 0$$

$$(x - 1)(x - 5)$$

c)

$$x^2 - 9x + 14 = 0$$

$$(x - 2)(x - 7)$$

d)

$$x^2 - 7x + 12 = 0$$

$$(x - 3)(x - 4)$$

e)

$$x^2 - 11x + 24 = 0$$

$$(x - 3)(x - 8)$$

f)

$$x^2 - 11x + 30 = 0$$

$$(x - 5)(x - 6)$$

3. Mixed Signs (Positive Dominant)

Negative constant \rightarrow mixed signs. Linear term positive \rightarrow the positive factor dominates.

a)

$$x^2 - 4x - 5 = 0$$

$$(x + 1)(x - 5)$$

b)

$$x^2 - 5x - 14 = 0$$

$$(x + 2)(x - 7)$$

c)

$$x^2 - 5x - 24 = 0$$

$$(x + 3)(x - 8)$$

d)

$$x^2 - 5x - 36 = 0$$

$$(x + 4)(x - 9)$$

e)

$$x^2 - 6x - 55 = 0$$

$$(x + 5)(x - 11)$$

f)

$$x^2 - 6x - 91 = 0$$

$$(x + 7)(x - 13)$$

4. Mixed Signs (Negative Dominant)

Negative constant \rightarrow mixed signs. Linear term negative \rightarrow the negative factor dominates.

a)

$$x^2 + 4x - 5 = 0$$

$$(x + 5)(x - 1)$$

b)

$$x^2 + 6x - 7 = 0$$

$$(x + 7)(x - 1)$$

c)

$$x^2 + 6x - 16 = 0$$

$$(x + 8)(x - 2)$$

d)

$$x^2 + 6x - 27 = 0$$

$$(x + 9)(x - 3)$$

e)

$$x^2 + 7x - 44 = 0$$

$$(x + 11)(x - 4)$$

f)

$$x^2 + 8x - 65 = 0$$

$$(x + 13)(x - 5)$$

5. **24 Mixed Jumbled Questions**

A full mix of all four sign-patterns.

1)

$$x^2 - 1x - 2 = 0$$

$$(x + 1)(x - 2)$$

2)

$$x^2 + 2x - 3 = 0$$

$$(x + 3)(x - 1)$$

3)

$$x^2 - 12x + 35 = 0$$

$$(x - 5)(x - 7)$$

4)

$$x^2 - 6x - 55 = 0$$

$$(x + 5)(x - 11)$$

5)

$$x^2 - 14x + 13 = 0$$

$$(x - 1)(x - 13)$$

6)

$$x^2 + 6x - 7 = 0$$

$$(x + 7)(x - 1)$$

7)

$$x^2 - 14x + 33 = 0$$

$$(x - 3)(x - 11)$$

8)

$$x^2 + 9x - 22 = 0$$

$$(x + 11)(x - 2)$$

9)

$$x^2 - 12x - 13 = 0$$

$$(x + 1)(x - 13)$$

10)

$$x^2 - 7x + 10 = 0$$

$$(x - 2)(x - 5)$$

11)

$$x^2 - 4x - 21 = 0$$

$$(x + 3)(x - 7)$$

12)

$$x^2 + 3x - 10 = 0$$

$$(x + 5)(x - 2)$$

13)

$$x^2 - 16x + 55 = 0$$

$$(x - 5)(x - 11)$$

14)

$$x^2 + 4x - 21 = 0$$

$$(x + 7)(x - 3)$$

15)

$$x^2 - 8x + 7 = 0$$

$$(x - 1)(x - 7)$$

16)

$$x^2 + 6x - 55 = 0$$

$$(x + 11)(x - 5)$$

17)

$$x^2 + 12x - 13 = 0$$

$$(x + 13)(x - 1)$$

18)

$$x^2 - 16x + 39 = 0$$

$$(x - 3)(x - 13)$$

19)

$$x^2 - 9x - 22 = 0$$

$$(x + 2)(x - 11)$$

20)

$$x^2 - 18x + 77 = 0$$

$$(x - 7)(x - 11)$$

21)

$$x^2 + 4x - 5 = 0$$

$$(x + 5)(x - 1)$$

22)

$$x^2 - 2x - 15 = 0$$

$$(x + 3)(x - 5)$$

23)

$$x^2 - 15x + 26 = 0$$

$$(x - 2)(x - 13)$$

24)

$$x^2 + 5x - 14 = 0$$

$$(x + 7)(x - 2)$$